@prefix rdf: <http://www.w3.org/1999/02/22-rdf-syntax-ns#> .
@prefix gbv: <http://purl.org/ontology/gbv#> .
@prefix cc: <http://creativecommons.org/ns#> .
@prefix daia: <http://purl.org/ontology/daia/> .
@prefix dct: <http://purl.org/dc/terms/> .
@prefix owl: <http://www.w3.org/2002/07/owl#> .
@prefix rdfs: <http://www.w3.org/2000/01/rdf-schema#> .
@prefix skos: <http://www.w3.org/2004/02/skos/core#> .
@prefix vann: <http://purl.org/vocab/vann/> .
@prefix voaf: <http://purl.org/vocommons/voaf#> .
@prefix void: <http://rdfs.org/ns/void#> .
@prefix vs: <http://www.w3.org/2003/06/sw-vocab-status/ns#> .
@prefix xsd: <http://www.w3.org/2001/XMLSchema#> .

<http://purl.org/ontology/gbv>
    cc:license <http://creativecommons.org/licenses/by/3.0/> ;
    dct:creator "Jakob Vo√ü" ;
    dct:description "Ontology of common concepts and relationships used in the GBV library network" ;
    dct:modified "2014-06-30"^^xsd:date ;
    dct:title "GBV Ontology" ;
    vann:preferredNamespacePrefix "gbv" ;
    vann:preferredNamespaceUri "http://purl.org/ontology/gbv#" ;
    a voaf:Vocabulary, owl:Ontology ;
    rdfs:label "GBV" ;
    owl:versionInfo "rev3" .

gbv:dbkey
    a owl:DatatypeProperty ;
    rdfs:comment "database key, used as prefix in unAPI and at other APIs within the GBV"@en ;
    rdfs:isDefinedBy <http://purl.org/ontology/gbv#> ;
    rdfs:label "dbkey"@en ;
    rdfs:subPropertyOf dct:identifier ;
    skos:scopeNote "must comply to the regular expression ^[a-z][a-z0-9-]*[a-z0-9]$"@en .

gbv:eln
    a owl:DatatypeProperty ;
    rdfs:comment "external library number (ELN) as library identifier within the GBV"@en ;
    rdfs:isDefinedBy <http://purl.org/ontology/gbv#> ;
    rdfs:label "eln"@en ;
    rdfs:subPropertyOf dct:identifier .

gbv:gvkppn
    a owl:DatatypeProperty ;
    rdfs:comment "PPN identifier within the GBV union catalog (GVK)"@en ;
    rdfs:isDefinedBy <http://purl.org/ontology/gbv#> ;
    rdfs:label "gvkppn"@en ;
    rdfs:subPropertyOf dct:identifier ;
    skos:scopeNote "a PPN in general identifies a record in any PICA database. This property must only be used to identity records in GVK."@en .

gbv:iln
    a owl:DatatypeProperty ;
    rdfs:comment "internal library number (ILN) as library identifier within the GBV"@en ;
    rdfs:isDefinedBy <http://purl.org/ontology/gbv#> ;
    rdfs:label "iln"@en ;
    rdfs:subPropertyOf dct:identifier .

gbv:oaibase
    a owl:ObjectProperty ;
    rdfs:comment "OAI-PMH base URL of a database"@en ;
    rdfs:domain void:Dataset ;
    rdfs:isDefinedBy <http://purl.org/ontology/gbv#> ;
    rdfs:label "oaibase"@en .

gbv:opac
    a owl:ObjectProperty ;
    rdfs:comment "main catalog of an institution"@en ;
    rdfs:domain daia:Institution ;
    rdfs:isDefinedBy <http://purl.org/ontology/gbv#> ;
    rdfs:label "opac"@en ;
    rdfs:range void:Dataset ;
    rdfs:seeAlso <http://id.loc.gov/vocabulary/relators/own>, <http://purl.org/cld/terms/catalogueOrIndex> ;
    skos:scopeNote "the main catalog of a library usually contains records about its holdings, but the main catalog could also contain records that are not held by the institution."@en .

gbv:picabase
    a owl:ObjectProperty ;
    rdfs:comment "PICA base URL of a database"@en ;
    rdfs:domain void:Dataset ;
    rdfs:isDefinedBy <http://purl.org/ontology/gbv#> ;
    rdfs:label "picabase"@en .

gbv:ppn
    a rdfs:Datatype ;
    rdfs:comment "A PPN in general identifies a record in a PICA database, but it does not indicate which database it comes from."@en ;
    rdfs:isDefinedBy <http://purl.org/ontology/gbv#> ;
    rdfs:label "PPN identifier"@en .

gbv:solrbase
    a owl:ObjectProperty ;
    rdfs:comment "Solr base URL of a database"@en ;
    rdfs:domain void:Dataset ;
    rdfs:isDefinedBy <http://purl.org/ontology/gbv#> ;
    rdfs:label "solrbase"@en .

gbv:srubase
    a owl:ObjectProperty ;
    rdfs:comment "SRU interface of a database"@en ;
    rdfs:domain void:Dataset ;
    rdfs:isDefinedBy <http://purl.org/ontology/gbv#> ;
    rdfs:label "srubase"@en .

